fixed formatting of the other benchmark programs thus far

tasks/fill_body/MeanAbsoluteDeviationNonnegative_fillbody.dfy
@@ -4,6 +4,10 @@ For a given list of input numbers, calculate Mean Absolute Deviation around the 
 Mean Absolute Deviation is the average absolute difference between each element and a centerpoint (mean in this case): 
 MAD = average | x - x_mean |
 */
+function abs(x: real): real
+{
+  /* TODO */
+}
 
 function sum(numbers: seq<real>): real
 {
@@ -17,6 +21,13 @@ function mean(numbers: seq<real>): real
     requires numbers != []
 {
     sum(numbers) / (|numbers| as real)
+}
+
+function mapf<A,B>(f: A -> B, xs: seq<A>): seq<B>
+    ensures |xs| == |mapf(f, xs)|
+    ensures forall i :: 0 <= i < |xs| ==> (mapf(f, xs))[i] == f(xs[i])
+{
+    /* TODO */
 }
 
 function mean_absolute_deviation(numbers: seq<real>):real
@@ -39,7 +50,7 @@ lemma mean_nonnegative(numbers: seq<real>)
     /* TODO */
 }
 
-lemma mean_absolute_deviation_nonnegative(numbers: seq<real>)
+lemma MeanAbsoluteDeviationNonnegative(numbers: seq<real>)
     requires numbers != []
     ensures mean_absolute_deviation(numbers) >= 0.0
 {
