programs/HasCloseElements _variant01.dfy
@@ -3,7 +3,7 @@ HumanEvalX 0 - Clover variant
 Check if in given list of numbers, are any two numbers closer to each other than given threshold.
 */
 
-method has_close_elements(numbers: seq<real>, threshold: real) returns (res: bool)
+method HasCloseElements_variant01(numbers: seq<real>, threshold: real) returns (res: bool)
   requires threshold >= 0.0
   ensures res ==> exists i: int, j: int :: 0 <= i < |numbers| && 0 <= j < |numbers| && i != j && (if numbers[i] - numbers[j] < 0.0 then numbers[j] - numbers[i] else numbers[i] - numbers[j]) < threshold
   ensures !res ==> (forall i: int, j: int :: 1 <= i < |numbers| && 0 <= j < i ==>  (if numbers[i] - numbers[j] < 0.0 then numbers[j] - numbers[i] else numbers[i] - numbers[j]) >= threshold)
