programs/HasCloseElements.dfy
@@ -8,7 +8,7 @@ function abs(x: real): real
   if x < 0.0 then -x else x
 }
 
-method has_close_elements(numbers: seq<real>, threshold: real) returns (result: bool)
+method HasCloseElements(numbers: seq<real>, threshold: real) returns (result: bool)
     ensures result <==> exists i, j ::
       0 <= i < |numbers| &&
       0 <= j < |numbers| &&
