programs/RollingMax.dfy
@@ -24,7 +24,7 @@ ensures isMax(result, numbers)
     }
 }
 
-method rolling_max(numbers: seq<int>) returns (result: seq<int>)
+method RollingMax(numbers: seq<int>) returns (result: seq<int>)
 requires numbers != []
 ensures |result| == |numbers|
 ensures forall i :: 0 < i < |result| ==> isMax(result[i], numbers[0..(i+1)])
