tasks/fill_body/RollingMax_fillbody.dfy
@@ -10,7 +10,14 @@ function isMax(m: int, numbers: seq<int>): bool
 
 }
 
-method rolling_max(numbers: seq<int>) returns (result: seq<int>)
+method max(numbers: seq<int>) returns (result: int)
+requires numbers != []
+ensures isMax(result, numbers)
+{
+    /* TODO */
+}
+
+method RollingMax(numbers: seq<int>) returns (result: seq<int>)
 requires numbers != []
 ensures |result| == |numbers|
 ensures forall i :: 0 < i < |result| ==> isMax(result[i], numbers[0..(i+1)])
